src/dvspec/dafny/att_spec_proofs/inv33.dfy
@@ -227,9 +227,9 @@ module Inv33
     requires inv1(s)
     requires inv53(s)
     requires inv3(s)    
-    requires inv33(s)
-    requires inv_attestation_consensus_active_instances_keys_is_subset_of_att_slashing_db_hist(s)
     requires hn in s.honest_nodes_states.Keys
+    requires inv33_body(s, hn, s.honest_nodes_states[hn], cid)
+    requires inv_attestation_consensus_active_instances_keys_is_subset_of_att_slashing_db_hist(s)
     ensures inv33_body(s', hn, s'.honest_nodes_states[hn], cid)
     {
         assert s.att_network.allMessagesSent <= s'.att_network.allMessagesSent;
@@ -356,7 +356,7 @@ module Inv33
                     ==> s in hn_state.attestation_consensus_engine_state.att_slashing_db_hist.Keys)
                 ;
         }
-    }     
+    }  
 
     lemma lemma_inv_46_a(
         s: DVState,
@@ -374,5 +374,353 @@ module Inv33
     {
         lemma_inv_33(s, event, s');
         lemma_inv33_implies_46_a(s');
+    }     
+
+    lemma lemma_add_set_of_validity_predicates<D(!new, 0)>(
+        existing_honest_nodes_validity_predicates: map<BLSPubkey, set<D -> bool>>,
+        honest_nodes_validity_predicates: map<BLSPubkey, D -> bool>,
+        new_honest_nodes_validity_predicates: map<BLSPubkey, set<D -> bool>>
+    )
+    requires new_honest_nodes_validity_predicates == add_set_of_validity_predicates(existing_honest_nodes_validity_predicates, honest_nodes_validity_predicates)
+    ensures new_honest_nodes_validity_predicates.Keys == existing_honest_nodes_validity_predicates.Keys + new_honest_nodes_validity_predicates.Keys
+    {
+
+    }
+
+    lemma lemma_add_set_of_validity_predicates2<D(!new, 0)>(
+        existing_honest_nodes_validity_predicates: map<BLSPubkey, set<D -> bool>>,
+        honest_nodes_validity_predicates: map<BLSPubkey, D -> bool>,
+        new_honest_nodes_validity_predicates: map<BLSPubkey, set<D -> bool>>,
+        n: BLSPubkey,
+        vp: D -> bool
+    )
+    requires new_honest_nodes_validity_predicates == add_set_of_validity_predicates(existing_honest_nodes_validity_predicates, honest_nodes_validity_predicates)
+    ensures new_honest_nodes_validity_predicates.Keys == existing_honest_nodes_validity_predicates.Keys + new_honest_nodes_validity_predicates.Keys
+    requires n in existing_honest_nodes_validity_predicates.Keys
+    requires vp !in existing_honest_nodes_validity_predicates[n]
+    requires vp in new_honest_nodes_validity_predicates[n]
+    ensures vp == honest_nodes_validity_predicates[n]
+    {
+
+    }    
+
+    lemma lemma_add_set_of_validity_predicates3<D(!new, 0)>(
+        existing_honest_nodes_validity_predicates: map<BLSPubkey, set<D -> bool>>,
+        honest_nodes_validity_predicates: map<BLSPubkey, D -> bool>,
+        new_honest_nodes_validity_predicates: map<BLSPubkey, set<D -> bool>>,
+        n: BLSPubkey,
+        vp: D -> bool
+    )
+    requires new_honest_nodes_validity_predicates == add_set_of_validity_predicates(existing_honest_nodes_validity_predicates, honest_nodes_validity_predicates)
+    ensures new_honest_nodes_validity_predicates.Keys == existing_honest_nodes_validity_predicates.Keys + new_honest_nodes_validity_predicates.Keys
+    requires n !in existing_honest_nodes_validity_predicates
+    requires n in honest_nodes_validity_predicates
+    requires vp in new_honest_nodes_validity_predicates[n]
+    ensures vp == honest_nodes_validity_predicates[n]
+    {
+
     }      
+
+    function lemma_inv_46_b_ii_helper_helper_function(
+        s_w_honest_node_states_updated: DVState,
+        cid: Slot
+    ) : map<BLSPubkey, AttestationData -> bool>
+    {
+        map n |
+                && n in s_w_honest_node_states_updated.honest_nodes_states.Keys 
+                && cid in s_w_honest_node_states_updated.honest_nodes_states[n].attestation_consensus_engine_state.attestation_consensus_active_instances.Keys
+            ::
+                s_w_honest_node_states_updated.honest_nodes_states[n].attestation_consensus_engine_state.attestation_consensus_active_instances[cid].validityPredicate
+    }    
+
+    // lemma lemma_inv_46_b_ii_helper_helper(
+    //     s_w_honest_node_states_updated: DVState,
+    //     cid: Slot,
+    //     validityPredicates: map<BLSPubkey, AttestationData -> bool>,
+    //     n: BLSPubkey
+    // ) 
+    // requires validityPredicates == lemma_inv_46_b_ii_helper_helper_function(s_w_honest_node_states_updated, cid)
+    // requires n in validityPredicates.Keys
+    // // ensures validityPredicates[n] == s_w_honest_node_states_updated.honest_nodes_states[n].attestation_consensus_engine_state.attestation_consensus_active_instances[cid].validityPredicate
+    // {
+
+    // }  
+
+    // // lemma lemma_inv_46_b_ii_helper_helper2(
+    // //     s_w_honest_node_states_updated: DVState,
+    // //     cid: Slot,
+    // //     validityPredicates: map<BLSPubkey, AttestationData -> bool>,
+    // //     n: BLSPubkey
+    // // ) 
+    // // requires validityPredicates == lemma_inv_46_b_ii_helper_helper_function(s_w_honest_node_states_updated, cid)
+    // // requires n in validityPredicates.Keys
+    // // requires n !in s_w_honest_node_states_updated.honest_nodes_states
+    // // ensures cid in 
+    // // // ensures validityPredicates[n] == s_w_honest_node_states_updated.honest_nodes_states[n].attestation_consensus_engine_state.attestation_consensus_active_instances[cid].validityPredicate
+    // // {
+
+    // // }    
+
+    // lemma lemma_att_slashing_db_hist_cid_is_monotonic_f_check_for_next_queued_duty_rec(
+    //     s: DVCNodeState,
+    //     s': DVCNodeState,
+    //     cid: Slot
+    // )
+    // requires f_check_for_next_queued_duty.requires(s)
+    // requires s' == f_check_for_next_queued_duty(s).state
+    // requires cid in s.attestation_consensus_engine_state.att_slashing_db_hist.Keys
+    // ensures cid in s'.attestation_consensus_engine_state.att_slashing_db_hist.Keys
+    // ensures s.attestation_consensus_engine_state.att_slashing_db_hist[cid].Keys <= s'.attestation_consensus_engine_state.att_slashing_db_hist[cid].Keys; 
+
+    // lemma lemma_att_slashing_db_hist_cid_is_monotonic_f_check_for_next_queued_duty(
+    //     s: DVCNodeState,
+    //     s': DVCNodeState,
+    //     cid: Slot
+    // )
+    // requires f_check_for_next_queued_duty.requires(s)
+    // requires s' == f_check_for_next_queued_duty(s).state
+    // requires inv_attestation_consensus_active_instances_keys_is_subset_of_att_slashing_db_hist_body_body(s)
+    // requires cid in s.attestation_consensus_engine_state.att_slashing_db_hist.Keys
+    // ensures cid in s'.attestation_consensus_engine_state.att_slashing_db_hist.Keys
+    // // ensures s.attestation_consensus_engine_state.att_slashing_db_hist[cid].Keys <= s'.attestation_consensus_engine_state.att_slashing_db_hist[cid].Keys; 
+    // decreases s.attestation_duties_queue
+    // {
+    //     if  && s.attestation_duties_queue != [] 
+    //         && (
+    //             || s.attestation_duties_queue[0].slot in s.future_att_consensus_instances_already_decided
+    //             || !s.current_attestation_duty.isPresent()
+    //         )    
+    //     {
+            
+    //         if s.attestation_duties_queue[0].slot in s.future_att_consensus_instances_already_decided.Keys 
+    //         {
+    //             var queue_head := s.attestation_duties_queue[0];
+    //             var new_attestation_slashing_db := f_update_attestation_slashing_db(s.attestation_slashing_db, s.future_att_consensus_instances_already_decided[queue_head.slot]);
+    //             var s_mod := s.(
+    //                 attestation_duties_queue := s.attestation_duties_queue[1..],
+    //                 future_att_consensus_instances_already_decided := s.future_att_consensus_instances_already_decided - {queue_head.slot},
+    //                 attestation_slashing_db := new_attestation_slashing_db,
+    //                 attestation_consensus_engine_state := updateConsensusInstanceValidityCheck(
+    //                     s.attestation_consensus_engine_state,
+    //                     new_attestation_slashing_db
+    //                 )                        
+    //             );
+    //             lemma_pred_4_1_g_iii_f_check_for_next_queued_duty_updateConsensusInstanceValidityCheck5(
+    //                 s.attestation_consensus_engine_state,
+    //                 new_attestation_slashing_db,
+    //                 s_mod.attestation_consensus_engine_state,
+    //                 cid
+    //             );
+    //             assert s.attestation_consensus_engine_state.att_slashing_db_hist.Keys <= s_mod.attestation_consensus_engine_state.att_slashing_db_hist.Keys;
+    //             lemma_att_slashing_db_hist_cid_is_monotonic_f_check_for_next_queued_duty_rec(s_mod, s', cid);
+    //             assert s.attestation_consensus_engine_state.att_slashing_db_hist[cid].Keys <= s'.attestation_consensus_engine_state.att_slashing_db_hist[cid].Keys; 
+    //         }
+    //         else
+    //         {
+    //             // assert cid !in s.attestation_consensus_engine_state.attestation_consensus_active_instances.Keys;
+    //             assert s.attestation_duties_queue[0].slot !in s.attestation_consensus_engine_state.attestation_consensus_active_instances.Keys;
+
+    //         }
+    //     }
+    // }      
+
+    lemma lemma_att_slashing_db_hist_cid_is_monotonic(
+        s: DVCNodeState,
+        event: Types.Event,
+        s': DVCNodeState,
+        outputs: Outputs,
+        cid: Slot       
+    )
+    requires DVCNode_Spec.Next(s, event, s', outputs)
+    requires cid in s.attestation_consensus_engine_state.att_slashing_db_hist.Keys
+    ensures cid in s'.attestation_consensus_engine_state.att_slashing_db_hist.Keys
+    ensures s.attestation_consensus_engine_state.att_slashing_db_hist[cid].Keys <= s'.attestation_consensus_engine_state.att_slashing_db_hist[cid].Keys;   
+
+    lemma lemma_att_slashing_db_hist_cid_is_monotonic_corollary(
+        s: DVCNodeState,
+        event: Types.Event,
+        s': DVCNodeState,
+        outputs: Outputs,
+        cid: Slot,
+        vp: AttestationData -> bool       
+    )
+    requires DVCNode_Spec.Next(s, event, s', outputs)
+    requires cid in s.attestation_consensus_engine_state.att_slashing_db_hist.Keys
+    requires vp in s.attestation_consensus_engine_state.att_slashing_db_hist[cid]
+    ensures cid in s'.attestation_consensus_engine_state.att_slashing_db_hist.Keys
+    ensures vp in s'.attestation_consensus_engine_state.att_slashing_db_hist[cid]
+    {
+        lemma_att_slashing_db_hist_cid_is_monotonic(s, event, s', outputs, cid);
+    }          
+
+    lemma lemma_inv_46_b_ii_helper(
+        s: DVState,
+        event: DV.Event,
+        cid: Slot,
+        vp: AttestationData -> bool,
+        hn: BLSPubkey,
+        s': DVState
+    )
+    requires NextEvent(s, event, s')
+    requires inv1(s)
+    requires inv53(s)
+    requires inv3(s)    
+    requires hn in s.honest_nodes_states.Keys
+    requires inv33_body(s, hn, s.honest_nodes_states[hn], cid)
+    requires inv46_b_ii_body(s, hn, s.honest_nodes_states[hn], cid, vp)
+    requires inv_attestation_consensus_active_instances_keys_is_subset_of_att_slashing_db_hist(s)
+    requires inv_attestation_consensus_active_instances_predicate_is_in_att_slashing_db_hist_body(s.honest_nodes_states[hn], cid)
+    ensures inv46_b_ii_body(s', hn, s'.honest_nodes_states[hn], cid, vp)
+    {
+        // lemma_inv_33_helper(s, event, cid, hn, s');
+        assert s.att_network.allMessagesSent <= s'.att_network.allMessagesSent;
+        match event 
+        {
+            
+            case HonestNodeTakingStep(node, nodeEvent, nodeOutputs) =>
+
+                var s_w_honest_node_states_updated := lemma_pred_4_1_f_g_i_get_s_w_honest_node_states_updated(s, node, nodeEvent);           
+
+                assert s_w_honest_node_states_updated.consensus_on_attestation_data == s.consensus_on_attestation_data;
+
+
+                var output := 
+                    if nodeEvent.AttConsensusDecided? && nodeEvent.id == cid then 
+                        Some(Decided(node, nodeEvent.decided_attestation_data))
+                    else
+                        None
+                    ;
+
+                var validityPredicates := lemma_inv_46_b_ii_helper_helper_function(s_w_honest_node_states_updated, cid);
+                    // map n |
+                    //         && n in s_w_honest_node_states_updated.honest_nodes_states.Keys 
+                    //         && cid in s_w_honest_node_states_updated.honest_nodes_states[n].attestation_consensus_engine_state.attestation_consensus_active_instances.Keys
+                    //     ::
+                    //         s_w_honest_node_states_updated.honest_nodes_states[n].attestation_consensus_engine_state.attestation_consensus_active_instances[cid].validityPredicate
+                    // ;
+
+                var s_consensus := s_w_honest_node_states_updated.consensus_on_attestation_data[cid];
+                var s'_consensus := s'.consensus_on_attestation_data[cid];                
+
+                assert
+                    ConsensusSpec.Next(
+                        s_consensus,
+                        validityPredicates,
+                        s'_consensus,
+                        output
+                    );
+                
+                var hn_state := s.honest_nodes_states[hn];
+                var hn'_state := s'.honest_nodes_states[hn];
+
+                if 
+                    && hn in s'.consensus_on_attestation_data[cid].honest_nodes_validity_functions.Keys
+                    && vp in s'.consensus_on_attestation_data[cid].honest_nodes_validity_functions[hn]                          
+                    && cid in hn'_state.attestation_consensus_engine_state.att_slashing_db_hist.Keys
+          
+                   
+                {
+                    // assert s'_consensus.honest_nodes_validity_functions == add_set_of_validity_predicates(s_consensus.honest_nodes_validity_functions, validityPredicates);
+                    if hn in  s.consensus_on_attestation_data[cid].honest_nodes_validity_functions.Keys
+                    {
+                        if vp in s.consensus_on_attestation_data[cid].honest_nodes_validity_functions[hn]
+                        {
+                            assert cid in hn'_state.attestation_consensus_engine_state.att_slashing_db_hist.Keys;
+                            assert vp in hn_state.attestation_consensus_engine_state.att_slashing_db_hist[cid];
+                        }
+                        else 
+                        {
+                            lemma_add_set_of_validity_predicates2(
+                                s_consensus.honest_nodes_validity_functions, 
+                                validityPredicates,
+                                s'_consensus.honest_nodes_validity_functions,
+                                hn,
+                                vp
+                            );
+                            assert vp == s.honest_nodes_states[hn].attestation_consensus_engine_state.attestation_consensus_active_instances[cid].validityPredicate; 
+                            assert vp in hn_state.attestation_consensus_engine_state.att_slashing_db_hist[cid];
+                        }
+                    }
+                    else 
+                    {
+                        assert hn in validityPredicates;
+                        assert hn !in  s_consensus.honest_nodes_validity_functions.Keys;
+                        // assert cid in s.honest_nodes_states[hn].attestation_consensus_engine_state.attestation_consensus_active_instances.Keys;
+                        // assert vp == s.honest_nodes_states[hn].attestation_consensus_engine_state.attestation_consensus_active_instances[cid].validityPredicate; 
+                        
+                        lemma_add_set_of_validity_predicates3(
+                            s_consensus.honest_nodes_validity_functions, 
+                            validityPredicates,
+                            s'_consensus.honest_nodes_validity_functions,
+                            hn,
+                            vp
+                        );
+
+                        assert vp == s.honest_nodes_states[hn].attestation_consensus_engine_state.attestation_consensus_active_instances[cid].validityPredicate; 
+                        assert vp in hn_state.attestation_consensus_engine_state.att_slashing_db_hist[cid];
+
+                    }
+                    assert vp in hn_state.attestation_consensus_engine_state.att_slashing_db_hist[cid];
+
+                    if hn == node 
+                    {
+                        assert DVCNode_Spec.Next(s_w_honest_node_states_updated.honest_nodes_states[hn], nodeEvent, s'.honest_nodes_states[hn], nodeOutputs);
+                        lemma_att_slashing_db_hist_cid_is_monotonic_corollary(s_w_honest_node_states_updated.honest_nodes_states[hn], nodeEvent, s'.honest_nodes_states[hn], nodeOutputs, cid, vp);
+                        // assert s_w_honest_node_states_updated.honest_nodes_states[hn].attestation_consensus_engine_state.att_slashing_db_hist.Keys <= s'.honest_nodes_states[hn].attestation_consensus_engine_state.att_slashing_db_hist.Keys;
+                        // assert cid in s'.honest_nodes_states[hn].attestation_consensus_engine_state.att_slashing_db_hist.Keys;
+                        assert vp in hn'_state.attestation_consensus_engine_state.att_slashing_db_hist[cid];
+                    }
+                    else 
+                    {
+                        assert s.honest_nodes_states[hn] == s'.honest_nodes_states[hn];
+                        assert vp in hn'_state.attestation_consensus_engine_state.att_slashing_db_hist[cid];
+                    }   
+                    assert vp in hn'_state.attestation_consensus_engine_state.att_slashing_db_hist[cid];                 
+
+                }  
+
+                         
+            case AdeversaryTakingStep(node, new_attestation_share_sent, messagesReceivedByTheNode) => 
+                assert s'.consensus_on_attestation_data == s.consensus_on_attestation_data;
+                assert s.honest_nodes_states[hn] == s'.honest_nodes_states[hn];
+                 
+                if
+                    && hn in s'.consensus_on_attestation_data[cid].honest_nodes_validity_functions.Keys
+                    && vp in s'.consensus_on_attestation_data[cid].honest_nodes_validity_functions[hn]                          
+                    && cid in s'.honest_nodes_states[hn].attestation_consensus_engine_state.att_slashing_db_hist.Keys
+                {
+                    assert inv33_body(s, hn, s.honest_nodes_states[hn], cid);
+                    assert cid in s.honest_nodes_states[hn].attestation_consensus_engine_state.att_slashing_db_hist.Keys;
+                    assert s.honest_nodes_states[hn] == s'.honest_nodes_states[hn];
+                    assert cid in s'.honest_nodes_states[hn].attestation_consensus_engine_state.att_slashing_db_hist.Keys;
+                    assert vp in s'.honest_nodes_states[hn].attestation_consensus_engine_state.att_slashing_db_hist[cid];                 
+                    
+                } 
+
+        }
+    }  
+
+    lemma lemma_inv_46_b_ii(
+        s: DVState,
+        event: DV.Event,
+        s': DVState
+    )
+    requires NextEvent(s, event, s')
+    requires inv1(s)
+    requires inv53(s)
+    requires inv3(s)    
+    requires inv33(s)  
+    requires inv46_b_ii(s) 
+    requires inv_attestation_consensus_active_instances_keys_is_subset_of_att_slashing_db_hist(s)
+    requires inv_attestation_consensus_active_instances_predicate_is_in_att_slashing_db_hist(s)
+    ensures inv46_b_ii(s')   
+    {
+        forall hn: BLSPubkey, slot: Slot, vp : AttestationData -> bool |
+            hn in s'.honest_nodes_states
+        ensures inv46_b_ii_body(s', hn, s'.honest_nodes_states[hn], slot, vp)    
+        {
+            lemma_inv_46_b_ii_helper(s, event, slot, vp, hn, s');
+        }
+    }       
+
 }
